<?xml version="1.0" encoding="UTF-8" ?> 
<section xml:id="quadratics-quadratic-in-form" xmlns:xi="http://www.w3.org/2001/XInclude"> 
 
  <title> Quadratic in Form </title> 
 
  <introduction> <alert> Objective: Solve equations that are quadratic in form by substitution to create a quadratic equation. 
</alert> </introduction> 
 
   <p> 
We have seen three different ways to solve quadratics: factoring, completing the square, and the quadratic formula. A quadratic is any equation of the form <m>0=ax^2+bx+c</m>, however, we can use the skills learned to solve quadratics to solve problems with higher (or sometimes lower) powers if the equation is in what is called quadratic form. 
   </p> 

   <p> <alert>
Quadratic Form: <m>0=ax^m+bx^n+c</m> where <m>m=2n</m>
   </alert> </p> 

   <p>
An equation is in quadratic form if one of the exponents on a variable is double the exponent on the same variable somewhere else in the equation. If this is the case we can create a new variable, set it equal to the variable with smallest exponent. When we substitute this into the equation we will have a quadratic equation we can solve. 
</p>
  <p> <alert> World View Note:</alert> Arab mathematicians around the year <m>1000</m> were the first to use this method! 
 </p> 

  <example>
    <md> 
      <mrow> x^4-13x^2+36=0 \amp \quad  \text{Quadratic form, one exponent, $4$, double the other, $2$}  </mrow> 
      <mrow> y=x^2  \amp\quad  \text{New variable equal to the variable with smaller exponent}  </mrow> 
      <mrow> y^2=x^4 \amp\quad  \text{Square both sides}  </mrow> 
      <mrow> y^2-13y+36=0 \amp\quad  \text{Substitute} y \text{for} x^2 \text{ and} y^2 \text{for} x^4  </mrow> 
      <mrow> (y-9)(y-4)=0 \amp\quad  \text{Solve. We can solve this equation by factoring} </mrow> 
      <mrow> y-9=0 \text{ or } y-4=0  \amp\quad  \text{Set each factor equal to zero }  </mrow> 
      <mrow> \underline{+9 +9}  \qquad\underline{+4 +4} \amp\quad  \text{Solutions for $y$ , need $x$. We will use} y = x^2 \text{equation} </mrow> 
      <mrow> y=9 \text{ or } y=4 \amp\quad  \text{Solutions for $y$,
      need $x$. We will use }  y=x^2 \text{equation} </mrow> 
      <mrow>  9=x^2 \text{ or } 4=x^2 \amp\quad  \text{Substitute values for $y$}  </mrow> 
      <mrow>  \pm \sqrt{9}=\sqrt{x^2} \text{ or } \pm \sqrt{4}=\sqrt{x^2}      \amp\quad  \text{Solve using the even root property, simplify roots}  </mrow> 
      <mrow>  x= \pm 3, \pm 2 \amp\quad  \text{Our Solutions}  </mrow> 
</md>
</example> 

<p>
When we have higher powers of our variable, we could end up with many more solutions. The previous equation had four unique solutions.
</p>

  
  <example>
    <md> 
      <mrow> a^{-2}-a^{-1}-6=0   \amp \quad  \text{Quadratic form, one exponent, $- 2$, is double the other, $- 1$}   </mrow> 
      <mrow> b=a^{-1} \amp\quad  \text{Make a new variable equal to the variable with lowest exponent}  </mrow> 
      <mrow> b^2=a^{-2} \amp\quad  \text{Square both sides}  </mrow> 
      <mrow>  b^2-b-6=0   \amp \quad  \text{Substitute } b^2 \text{ for } a^{-2} \text{ and }  b \text{ for } a^{-1} </mrow> 
      <mrow> (b-3)(b+2)=0 \amp\quad  \text{Solve. We will solve by factoring} </mrow> 
      <mrow>  b-3=0 \text{ or } b+2=0  \amp\quad  \text{Set each factor equal to $0$}  </mrow> 
      <mrow>   \underline{+3 +3} \qquad \underline{-2 -2} \amp \quad  \text{Solve each equation}   </mrow> 
      <mrow>  b=3 \text{ or } b=-2  \amp\quad  \text{Solutions for
      $b$, still need $a$, substitute into } b = a^{-1} </mrow> 
      <mrow> 3=a^{-1} \text{ or } -2=a^{-1}   \amp\quad  \text{Raise both sides to $- 1$ power}  </mrow> 
      <mrow> 3^{-1}=a \text{ or } (-2)^{-1}   \amp \quad  \text{Simplify negative exponents}   </mrow> 
      <mrow> a= \frac{1}{3}, - \frac{1}{2}    \amp\quad  \text{Our Solution}  </mrow>
    </md>
  </example> 
 
  <p> 
 Just as with regular quadratics, these problems will not always have rational solutions. We also can have irrational or complex solutions to our equations. 
  </p> 

  <example>
    <md> 
     <mrow> 2x^4+x^2=6   \amp\quad  \text{Make equation equal to zero}  </mrow>
     <mrow>\underline{-6 -6} \amp\quad  \text{Subtract $6$ from both sides}  </mrow>
     <mrow>  2x^4+x^2-6=0  \amp\quad  \text{Quadratic form, one exponent, $4$, double the other, $2$ }  </mrow>
     <mrow>  y=x^2  \amp\quad  \text{New variable equal variable with smallest exponent}  </mrow>
     <mrow>  y^2=x^4  \amp\quad  \text{Square both sides}  </mrow>
     <mrow>  2y^2+y-6=0       \amp\quad  \text{Solve. We will factor this equation}  </mrow>
     <mrow>  (2y-3)(y+2)=0  \amp\quad  \text{Set each factor equal to zero}  </mrow>
     <mrow>  2y-3=0 \text{ or } y+2=0  \amp\quad  \text{Solve each equation}  </mrow>
     <mrow> \underline{+3 +3}\qquad \underline{-2 -2} </mrow>
     <mrow>   \frac{2y}{2}=\frac{3}{2} \text{ or } y=-2 </mrow>
     <mrow>  y=\frac{3}{2} \text{ or } y=-2   \amp\quad  \text{We have $y$, still need $x$. Substitute into }  y=x^2 </mrow>
     <mrow>  \frac{3}{2}=x^2 \text{ or } -2=x^2 \amp\quad  \text{Square root of each side}  </mrow>
     <mrow>  \pm \sqrt{\frac{3}{2}}=\sqrt{x^2} \text{ or } \pm \sqrt{-2}=\sqrt{x^2}    \amp\quad  \text{Simplify each root, rationalize denominator}  </mrow>
     <mrow>  x=\frac{\pm\sqrt{6}}{2}, \pm i\sqrt{2} \amp\quad  \text{Our Solution}  </mrow>
    </md>
  </example>
  
<p>
When we create a new variable for our substitution, it won’t always be equal to just another variable. We can make our substitution variable equal to an expression as shown in the next example.
</p>

<example> 
    <md>

      <mrow>  3(x-7)^2-2(x-7)+5=0  \amp\quad  \text{Quadratic Form}  </mrow>
      <mrow>  y=x-7  \amp\quad  \text{Define new variable}  </mrow>
      <mrow>  y^2=(x-7)^2  \amp\quad  \text{Square both sides}  </mrow>
      <mrow>  3y^2-2y+5=0  \amp\quad  \text{Substitute values into original}</mrow>
      <mrow>  (3y-5)(y+1)=0  \amp\quad  \text{Factor}  </mrow>
      <mrow> 3y-5=0 \text{ or } y+1=0  \amp\quad  \text{Set each factor equal to zero}  </mrow>
      <mrow>  \underline{+5 +5} \qquad\underline{-1 -1} \amp\quad  \text{Solve each equation}  </mrow>
      <mrow>  3y=5 \text{ or } y=-1  </mrow>
      <mrow>  \frac{3y}{3}=\frac{5}{3} \text{ or } y=-1  </mrow>
      <mrow>  y=\frac{5}{3} \text{ or } y=-1    \amp\quad  \text{We have $y$, we still need $x$}  </mrow>
      <mrow>  \frac{5}{3}=x-7 \text{ or } -1=x-7  \amp\quad \text{Substitute into } y=x-7  </mrow>
      <mrow> \underline{+\frac{21}{3} +7}\qquad\quad \underline{+7 \quad +7} \amp\quad  \text{Add $7$. Use common denominator as needed}  </mrow>
      <mrow>    x=\frac{26}{3}, 6 \amp\quad  \text{Our Solution}  </mrow>
    </md>
  </example> 


<example> 
    <md>
    <mrow> (x^2-6x)^2=7(x^2-6x)-12   \amp\quad  \text{Make equation equal zero} </mrow>
<mrow> -7(x^2-6x)+12-7(x^2-6x)+12    \amp\quad  \text{Move all terms to left} </mrow>
<mrow>  (x^2-6x)-7(x^2-6x)+12=0  \amp\quad  \text{Quadratic form} </mrow>
<mrow>  y=x^2-6x  \amp\quad  \text{Make new variable} </mrow>
<mrow> y^2=(x^2-6x)^2     \amp\quad  \text{Square both sides} </mrow>
<mrow>  y^2-7y+12=0  \amp\quad  \text{Substitute into original equation} </mrow>
<mrow>  (y-3)(y-4)=0  \amp\quad  \text{Solve by factoring} </mrow>  
<mrow> y-3=0 \text{ or } y-4=0  \amp\quad \text{ Set each factor equal to zero} </mrow>
<mrow> \underline{+3 +3} \qquad \underline{+4 +4}   \amp\quad  \text{ Solve each equation} </mrow>
<mrow>  y=3 \text{ or } y=4 \amp\quad  \text{We have $y$, still need $x$.} </mrow>
<mrow>  3=x^2-6x \text{ or }  4=x^3-6  \amp\quad  \text{Solve each equation, complete the square} </mrow>
<mrow>  (\frac{1}{2}\cdot 6)^2=3^2=9  \amp\quad  \text{Add $9$ to both sides of each equation} </mrow>
<mrow>  12=x^2-6x+9 \text{ or } 13=x^2-6x+9  \amp\quad  \text{Factor} </mrow>
<mrow> 12=(x-3)^2 \text{ or } 13=(x-3)^2   \amp\quad  \text{Use even root property} </mrow>
<mrow>  \pm\sqrt{12}=\sqrt{(x-3)^2} \text{ or } \pm\sqrt{13}=\sqrt{ (x-3)^2}   \amp\quad  \text{Simplify roots} </mrow>
<mrow>  \pm 2\sqrt{3}=x-3 \text{ or } \pm \sqrt{13}=x-3 \amp\quad  \text{Add $3$ to both sides} </mrow>
<mrow>  \underline{+3 \qquad +3} \qquad \underline{+3 \qquad +3}  \amp\quad  </mrow>
<mrow>  x=3 \pm 2\sqrt{3}, \ 3 \pm \sqrt{13}  \amp\quad  \text{Our Solution} </mrow>
    </md>
  </example> 

<p>
The higher the exponent, the more solution we could have. This is illustrated in the following example, one with six solutions.
</p>

<example>
  <md>
<mrow> x^6-9x^3+8=0   \amp\quad  \text{Quadratic form, one exponent, $6$, double the other, $3$} </mrow>
<mrow> y=x^3  \amp\quad  \text{New variable equal to variable with lowest exponent} </mrow>
<mrow> y^2=x^6   \amp\quad  \text{Square both sides} </mrow>
<mrow> y^2-9y+8=0  \amp\quad  \text{Substitute $y^2$ for $x^6$ and $y$
for } x^3 </mrow>
<mrow>  (y-1)(y-8)=0  \amp\quad  \text{Solve. We will solve by factoring. } </mrow>
<mrow>  y-1=0 \text{ or } y-8=0     \amp\quad  \text{Set each factor equal to zero} </mrow>
<mrow>\underline{+1 +1} \qquad \underline{+8 +8}  \amp\quad  \text{Solve each equation} </mrow>
<mrow>  y=1 \text{ or } y=8\amp\quad  \text{Solutions for $y$ , we need $x$. Substitute into} y = x^3 </mrow>
<mrow>  x^3=1 \text{ or } x^3=8  \amp\quad  \text{Set each equation equal to zero} </mrow>
<mrow>  \underline{-1 -1}\quad \underline{-8 -8}   </mrow>
<mrow> x^3-1=0 \text{ or } x^3-8=0   \amp\quad  \text{Factor each equation, difference of cubes} </mrow>
<mrow>  (x-1)(x^2+x+1)=0  \amp\quad  \text{First equation factored. Set each factor equal to zero} </mrow>
<mrow>  x-1=0 \text{ or } x^2+x+1=0    \amp\quad  \text{First equation is easy to solve} </mrow>
<mrow>   \underline{+1 +1}\qquad \qquad \qquad  \quad \amp\quad </mrow>
<mrow>  x=1 \qquad \qquad \qquad \quad \amp\quad  \text{First solution} </mrow>
<mrow>  \frac{-1 \pm \sqrt{1^2-4(1)(1)}}{2}=\frac{1 \pm i\sqrt{3}}{2}  \amp\quad  \text{Quadratic formula on second factor} </mrow>
<mrow>  (x-2)(x^2+2x+4)=0  \amp\quad  \text{Factor the second difference of cubes} </mrow>
<mrow>  x-2=0 \text{ or } x^2+2x+4=0  \amp\quad  \text{Set each factor equal to zero.} </mrow>
<mrow> \underline{+2 +2}\qquad \qquad \qquad  \qquad   \amp\quad  \text{First equation is easy to solve} </mrow>
<mrow> x=2  \qquad \qquad \qquad  \qquad  \amp\quad  \text{Our fourth solution} </mrow>
<mrow>  \frac{-2 \pm \sqrt{2^2-4(1)(4)}}{2(1)} =-1 \pm i\sqrt{3} \amp\quad  \text{Quadratic formula on second factor} </mrow>
<mrow> x=1, 2, \frac{1 \pm i\sqrt{3}}{2}, -1 \pm i\sqrt{3}   \amp\quad
\text{Our final six solutions} </mrow>
  </md>
  </example> 



<exercises xml:id="exercises-quadratic-in-form"> 
<title> Exercises – Quadratic in Form</title> 
<exercisegroup cols="2"> 
<introduction> 
<p> Solve each of the following equations. Some equations will have complex roots. </p> 
</introduction> 
<exercise><statement> <p> <m>x^{4} - 5x^{2} +4= 0 </m> </p> </statement></exercise>  
<exercise><statement> <p> <m>y^{4} - 9y^{2} + 20 = 0 </m> </p> </statement></exercise>
<exercise><statement> <p> <m>m^{4} - 7m^{2} - 8=0 </m> </p> </statement></exercise> 
<exercise><statement> <p> <m>y^{4} - 29y^{2} + 100 = 0 </m> </p> </statement></exercise>  
<exercise><statement> <p> <m>a^{4} - 50a^{2} + 49 =0 </m> </p> </statement></exercise>  
<exercise><statement> <p> <m>b^{4} - 10b^{2} + 9= 0 </m> </p> </statement></exercise>  
<exercise><statement> <p> <m>x^{4} - 25x^{2} + 144 = 0 </m> </p> </statement></exercise>  
<exercise><statement> <p> <m>y^{4} - 40y^{2} + 144 = 0 </m> </p> </statement></exercise>  
<exercise><statement> <p> <m>m^{4} - 20m^{2} + 64 = 0 </m> </p> </statement></exercise>  
<exercise><statement> <p> <m>x^{6} - 35x^{3} + 216 = 0 </m> </p> </statement></exercise>  
<exercise><statement> <p> <m>z^{6} - 216 = 19z^{3} </m> </p> </statement></exercise>  
<exercise><statement> <p> <m>y^{4} - 2y^{2} = 24 </m> </p> </statement></exercise>  
<exercise><statement> <p> <m>6z^{4} – z^{2} = 12 </m> </p> </statement></exercise>  
<exercise><statement> <p> <m>x^{-2} – x^{-1} - 12 = 0 </m> </p> </statement></exercise>  
<exercise><statement> <p> <m>x^{\frac{2}{3}} - 35 =2x^{\frac{1}{3}} </m> </p> </statement></exercise>  
<exercise><statement> <p> <m>5y^{-2} - 20 = 21y^{-1} </m> </p> </statement></exercise>  
<exercise><statement> <p> <m>y^{-6} + 7y^{-3} =8 </m> </p> </statement></exercise>  
<exercise><statement> <p> <m>x^{4}- 7x^{2} + 12 = 0 </m> </p> </statement></exercise>  
<exercise><statement> <p> <m>x^{4} - 2x^{2} - 3=0 </m> </p> </statement></exercise>  
<exercise><statement> <p> <m>x^{4} + 7x^{2} + 10 =0 </m> </p> </statement></exercise>  
<exercise><statement> <p> <m>2x^{4} - 5x^{2} + 2= 0 </m> </p> </statement></exercise>  
<exercise><statement> <p> <m>2x^{4} – x^{2} - 3=0 </m> </p> </statement></exercise>  
<exercise><statement> <p> <m>x^{4} - 9x^{2} +8= 0 </m> </p> </statement></exercise>  
<exercise><statement> <p> <m>x^{6} - 10x^{3} + 16 = 0 </m> </p> </statement></exercise>  
<exercise><statement> <p> <m>8x^{6} - 9x^{3} + 1= 0 </m> </p> </statement></exercise>  
<exercise><statement> <p> <m>8x^{6} + 7x^{3} - 1= 0 </m> </p> </statement></exercise>  
<exercise><statement> <p> <m>x^{8} - 17x^{4} + 16 = 0 </m> </p> </statement></exercise>  
<exercise><statement> <p> <m> (x - 1)^{2} - 4(x - 1)= 5 </m> </p> </statement></exercise>  
<exercise><statement> <p> <m> (y + b)^{2} - 4(y + b)= 21 </m> </p> </statement></exercise>  
<exercise><statement> <p> <m> (x +1)^{2} +6(x + 1)+ 9=0 </m> </p> </statement></exercise>  
<exercise><statement> <p> <m> (y + 2)^{2} - 6(y + 2)= 16 </m> </p> </statement></exercise>  
<exercise><statement> <p> <m> (m - 1)^{2} - 5(m - 1)= 14 </m> </p> </statement></exercise>  
<exercise><statement> <p> <m> (x - 3)^{2} - 2(x - 3)= 35 </m> </p> </statement></exercise>  
<exercise><statement> <p> <m> (a +1)^{2} +2(a - 1)= 15 </m> </p> </statement></exercise>  
<exercise><statement> <p> <m> (r - 1)^{2} - 8(r - 1) = 20 </m> </p> </statement></exercise>  
<exercise><statement> <p> <m>2(x - 1)^{2} - (x - 1)= 3 </m> </p> </statement></exercise>  
<exercise><statement> <p> <m>3(y + 1)^{2} - 14(y + 1) =5 </m> </p> </statement></exercise>  
<exercise><statement> <p> <m> (x^{2} - 3)^{2} - 2(x^{2} - 3)=3 </m> </p> </statement></exercise>  
<exercise><statement> <p> <m> (3x^{2} - 2x) 2 +5= 6(3x^{2} - 2x) </m> </p> </statement></exercise>  
<exercise><statement> <p> <m> (x^{2} + x +3)2 + 15 =8(x^{2} + x +3) </m> </p> </statement></exercise>  
<exercise><statement> <p> <m>2(3x +1)^{\frac{2}{3}} - 5(3x + 1)^{\frac{1}{3}} = 88 </m> </p> </statement></exercise>  
<exercise><statement> <p> <m> (x^{2} + x)^{2} - 8(x^{2} + x)+ 12 =0 </m> </p> </statement></exercise>  
<exercise><statement> <p> <m> (x^{2} + 2x)^{2} - 2(x^{2} +2x)=3 </m> </p> </statement></exercise>  
<exercise><statement> <p> <m> (2x^{2} + 3x)^{2} =8(2x^{2} +3x)+ 9 </m> </p> </statement></exercise>  
<exercise><statement> <p> <m> (2x^{2} - x)^{2} - 4(2x^{2} - x) + 3=0 </m> </p> </statement></exercise>  
<exercise><statement> <p> <m> (3x^{2} - 4x)^{2} =3(3x^{2} - 4x) + 4 </m> </p> </statement></exercise> 
</exercisegroup> 
 
      </exercises>
 
 
</section>

